TestVectors/runtimes/net/Generated/ESDK/TypeConversion.cs
@@ -459,12 +459,12 @@ namespace AWS.Cryptography.EncryptionSDK.Wrapped
                     );
                 // OpaqueError is redundant, but listed for completeness.
                 case OpaqueError exception:
-                    return new software.amazon.cryptography.encryptionsdk.internaldafny.types.Error_Opaque(exception);
+                    return new software.amazon.cryptography.encryptionsdk.internaldafny.types.Error_Opaque(exception, Dafny.Sequence<char>.FromString(exception.ToString()));
                 case System.Exception exception:
-                    return new software.amazon.cryptography.encryptionsdk.internaldafny.types.Error_Opaque(exception);
+                    return new software.amazon.cryptography.encryptionsdk.internaldafny.types.Error_Opaque(exception, Dafny.Sequence<char>.FromString(exception.ToString()));
                 default:
                     // The switch MUST be complete for System.Exception, so `value` MUST NOT be an System.Exception. (How did you get here?)
-                    return new software.amazon.cryptography.encryptionsdk.internaldafny.types.Error_Opaque(value);
+                    return new software.amazon.cryptography.encryptionsdk.internaldafny.types.Error_Opaque(value, Dafny.Sequence<char>.FromString(value.ToString()));
             }
         }
     }
